proofs/Axioms.lean
@@ -27,6 +27,9 @@ import Statements
 #print axioms Protocol.Statements.check_S14_window
 #print axioms Protocol.Statements.check_S14_queue
 #print axioms Protocol.Statements.check_S9_slot_body
+#print axioms Protocol.Statements.check_S18_restore_body
+#print axioms Protocol.Statements.check_S18_prepare
+#print axioms Protocol.Statements.check_S19_bound
 #print axioms Protocol.Statements.check_S12_prepare
 #print axioms Protocol.Statements.check_S12_bound
 #print axioms Protocol.Statements.check_S5_folder
